steel/Zeta.Steel.ApplicationTypes.fsti
@@ -66,7 +66,7 @@ val store_size : U16.t
 /// The number of verifier threads to use
 val n_threads : n:U32.t{ 0 < U32.v n /\ U32.v n < FStar.UInt.max_int 16 }
 
-let tid = n:U16.t { U16.v n < U32.v n_threads }
+let tid : eqtype = n:U16.t { U16.v n < U32.v n_threads }
 
 let app_args (fid:A.appfn_id aprm) =
   let fsig = Map.sel aprm.A.tbl fid in
